module Substitution where

open import Function hiding (_âˆ‹_)
open import Relation.Binary.PropositionalEquality as PropEq
  using (_â‰¡_; refl; sym; cong; congâ‚‚; cong-app)

open import STLC hiding (_âˆ)

------------------------------------------------------------------------------
-- Monad Laws for Parallel Substitution
-- 
-- T. Altenkirch and B. Reus, â€œMonadic Presentations of Lambda Terms Using Generalized Inductive Types,â€ in Computer Science Logic. CSL 1999, vol. 1683, J. Flum and M. Rodriguez-Artalejo, Eds. Springer, Berlin, Heidelberg, 1999, pp. 453â€“468. 
-- T. Altenkirch, J. Chapman, and T. Uustalu, â€œMonads need not be endofunctors,â€ LMCS, vol. 11, no. 1, pp. 1â€“40, 2015.

-- A relative monad on a functor J : ğ• â†’ â„‚ consits of
--   1. (monad)  a map on objects T : |ğ•| â†’ |â„‚|
--   2. (return) for any X âˆˆ |ğ•| a map Î·â‚“ : JX â†’ TX 
--   3. (bind)   for any X, Y âˆˆ |ğ•| and f : JX â†’ TY, a map f* : TX â†’ TY called the Kleisli extension of f.
-- satisfying the usual monad laws.

-- _âŠ¢_  is a relative monad formed by
--   1. ğ• = Obj : Context Type
--          Mor : (Ï : {A : Type} â†’ Î“ âˆ‹ A â†’ Î” âˆ‹ A)
-- 
--      equivalently, ğ•(Î“, Î”) = Rename Î“ Î”
--
--   2. â„‚ = [Type, Set] (in which Type is merely a discrete category) 
-- 
--                         f : ğ’« â‡’ ğ’¬
--                     ==========================
--                     f : {A : Type} â†’ ğ’« A â†’ ğ’¬ A
-- 
--   3. JÎ“ = Î“ âˆ‹_ : Type â†’ Set 
--      JÏ = Ï : âˆ€ {A} â†’ Î“ âˆ‹ A â†’ Î” âˆ‹ A
-- 
--   4. T: Context Type â†’ [Type, Set]
--                    Î“ â†¦ Î“ âŠ¢_
-- 
--   5. Î· = `_ : Î“ âˆ‹_ â‡’ Î“ âŠ¢_
-- 
--   6. Given Ïƒ âˆˆ â„‚(JÎ“, TÎ”) = Subst Î“ Î”, we have âŸª Ïƒ âŸ« : Î“ âŠ¢_ â‡’ Î” âŠ¢_ as the Kleisli extension, i.e.
-- 
--      Ïƒ : âˆ€ {A} â†’ Î“ âˆ‹ A â†’ Î” âŠ¢ A
--      -----------------------------
--      âŸª Ïƒ âŸ« : âˆ€ {A} â†’ Î“ âŠ¢ A â†’ Î” âŠ¢ A

infixr 5 _â¨Ÿ_

_â¨Ÿ_ : âˆ€{Î“ Î” Î£} â†’ Subst Î“ Î” â†’ Subst Î” Î£ â†’ Subst Î“ Î£
(Ïƒ â¨Ÿ Ï„) x = Ïƒ x âŸª Ï„ âŸ« 

ids : Subst Î“ Î“
ids = `_

----------------------------------------------------------------------
-- Congruence rules
rename-cong : {Ïâ‚ Ïâ‚‚ : Rename Î“ Î”}
  â†’ (âˆ€ {A} (x : Î“ âˆ‹ A) â†’ Ïâ‚ x â‰¡ Ïâ‚‚ x)
  â†’ (M : Î“ âŠ¢ A)
  â†’ rename Ïâ‚ M â‰¡ rename Ïâ‚‚ M
rename-cong p (` x)      = cong `_ (p x)
--rename-cong p (absurd A M) = cong (absurd A) (rename-cong p M)
rename-cong p (M Â· N)    =
  congâ‚‚ _Â·_ (rename-cong p M) (rename-cong p N)
rename-cong p (Æ› M)      =
  cong Æ›_ (rename-cong (Î» { Z â†’ refl ; (S x) â†’ cong S_ (p x)}) M)

subst-cong : {Ïƒâ‚ Ïƒâ‚‚ : Subst Î“ Î”}
  â†’ (âˆ€ {A} (x : Î“ âˆ‹ A) â†’ Ïƒâ‚ x â‰¡ Ïƒâ‚‚ x)
  â†’ (M : Î“ âŠ¢ A)
  â†’ M âŸª Ïƒâ‚ âŸ« â‰¡ M âŸª Ïƒâ‚‚ âŸ«
subst-cong p (` x)      = p x
--subst-cong p (absurd A M) = cong (absurd A) (subst-cong p M)
subst-cong p (M Â· N)    = congâ‚‚ _Â·_ (subst-cong p M) (subst-cong p N)
subst-cong p (Æ› M)      = cong Æ›_ (subst-cong 
  (Î» {Z â†’ refl ; (S x) â†’ cong (rename S_) (p x)}) M)

----------------------------------------------------------------------
-- Properties of ext 

ext-comp : (Ïâ‚ : Rename Î“ Î”) (Ïâ‚‚ : Rename Î” Î)
  â†’ (x : Î“ , B âˆ‹ A)
  â†’ (ext Ïâ‚‚ âˆ˜ ext Ïâ‚) x â‰¡ ext (Ïâ‚‚ âˆ˜ Ïâ‚) x
ext-comp Ïâ‚ Ïâ‚‚ Z     = refl
ext-comp Ïâ‚ Ïâ‚‚ (S x) = refl

----------------------------------------------------------------------
-- Properties of Rename

ren : Rename Î“ Î” â†’ Subst Î“ Î”
ren Ï = ids âˆ˜ Ï

rename=subst-ren
  : {Ï : Rename Î“ Î”}
  â†’ (M : Î“ âŠ¢ A)
  â†’ rename Ï M â‰¡ M âŸª ren Ï âŸ«
rename=subst-ren (` x)      = refl
--rename=subst-ren (absurd A M) = cong (absurd A) (rename=subst-ren M)
rename=subst-ren (M Â· N)    =
  congâ‚‚ _Â·_ (rename=subst-ren M) (rename=subst-ren N)
rename=subst-ren {Ï = Ï} (Æ› M)      = cong Æ›_ (begin
  rename (ext Ï) M
    â‰¡âŸ¨ rename=subst-ren M âŸ©
  M âŸª ren (ext Ï) âŸ«
    â‰¡âŸ¨ subst-cong (ren-ext Ï) M âŸ©
  M âŸª exts (ren Ï) âŸ«
    âˆ)
  where
    open PropEq.â‰¡-Reasoning
    ren-ext : (Ï : Rename Î“ Î”)
      â†’ âˆ€ {B} (x : Î“ , A âˆ‹ B) â†’ ren (ext Ï) x â‰¡ exts (ren Ï) x
    ren-ext Ï Z     = refl
    ren-ext Ï (S x) = refl

rename-comp
  : (Ïâ‚ : Rename Î“ Î”) (Ïâ‚‚ : Rename Î” Î)
  â†’ {M : Î“ âŠ¢ A}
  â†’ rename Ïâ‚‚ (rename Ïâ‚ M) â‰¡ rename (Ïâ‚‚ âˆ˜ Ïâ‚) M
rename-comp Ïâ‚ Ïâ‚‚ {M = ` x}      = refl
--rename-comp Ïâ‚ Ïâ‚‚ {M = absurd A M} = cong (absurd A) (rename-comp Ïâ‚ Ïâ‚‚)
rename-comp Ïâ‚ Ïâ‚‚ {M = M Â· N}    = congâ‚‚ _Â·_ (rename-comp Ïâ‚ Ïâ‚‚) (rename-comp Ïâ‚ Ïâ‚‚)
rename-comp Ïâ‚ Ïâ‚‚ {M = Æ› M}      = cong Æ›_ (begin
  rename (ext Ïâ‚‚) (rename (ext Ïâ‚) M)
    â‰¡âŸ¨ rename-comp (ext Ïâ‚) (ext Ïâ‚‚) âŸ©
  rename (ext Ïâ‚‚ âˆ˜ ext Ïâ‚) M
    â‰¡âŸ¨ rename-cong (ext-comp Ïâ‚ Ïâ‚‚) M âŸ©
  rename (ext (Ïâ‚‚ âˆ˜ Ïâ‚))   M
  âˆ)
  where open PropEq.â‰¡-Reasoning

----------------------------------------------------------------------
-- punchIn: Weakening at any position

punchIn : âˆ€ A {Î“â‚} Î“â‚‚ â†’ Rename (Î“â‚ â§º Î“â‚‚) (Î“â‚ , A â§º Î“â‚‚)
punchIn _ âˆ…       Z     = S Z
punchIn _ âˆ…       (S x) = S (S x)
punchIn _ (Î” , C) Z     = Z
punchIn _ (Î” , C) (S x) = S punchIn _ Î” x

punchesIn : âˆ€ Î â†’ Subst Î“ Î” â†’ Subst (Î“ â§º Î) (Î” â§º Î)
punchesIn âˆ…       Ïƒ x     = Ïƒ x
punchesIn (Î , C) Ïƒ Z     = ` Z
punchesIn (Î , C) Ïƒ (S x) = rename S_ (punchesIn Î Ïƒ x)

ext-punchIn=punchIn : (x : Î“ â§º Î , B âˆ‹ C)
  â†’ ext (punchIn A Î) x â‰¡ punchIn A (Î , B) x
ext-punchIn=punchIn {Î = âˆ…}     Z     = refl
ext-punchIn=punchIn {Î = âˆ…}     (S x) = refl
ext-punchIn=punchIn {Î = Î , B} Z     = refl
ext-punchIn=punchIn {Î = Î , B} (S x) = refl

exts-punchesIn=punchesIn : {Ïƒ : Subst Î“ Î”}
  â†’ (x : Î“ â§º Î , B âˆ‹ A)
  â†’ exts (punchesIn Î Ïƒ) x â‰¡ punchesIn (Î , B) Ïƒ x
exts-punchesIn=punchesIn Z     = refl
exts-punchesIn=punchesIn (S x) = refl

S=punchIn : (x : Î“ âˆ‹ A) â†’ S x â‰¡ punchIn B âˆ… x
S=punchIn Z     = refl
S=punchIn (S x) = refl

punchesIn-punchIn-comm : (Ïƒ : Subst Î“ Î”)
  â†’ (x : Î“ â§º Î âˆ‹ A)
  â†’ punchesIn Î (exts Ïƒ) (punchIn B Î x) â‰¡ rename (punchIn B Î) (punchesIn Î Ïƒ x)
punchesIn-punchIn-comm {Î = âˆ…}     Ïƒ Z     = rename-cong S=punchIn (Ïƒ Z)
punchesIn-punchIn-comm {Î = âˆ…}     Ïƒ (S x) = rename-cong S=punchIn (Ïƒ (S x))
punchesIn-punchIn-comm {Î = Î , C} Ïƒ Z     = refl
punchesIn-punchIn-comm {Î = Î , C} Ïƒ (S x) = begin
  rename S_ (punchesIn Î (exts Ïƒ) (punchIn _ Î x))
    â‰¡âŸ¨ cong (rename S_) (punchesIn-punchIn-comm Ïƒ x) âŸ©
  rename S_ (rename (punchIn _ Î) (punchesIn Î Ïƒ x))
    â‰¡âŸ¨ rename-comp (punchIn _ Î) S_ âŸ©
  rename (S_ âˆ˜ (punchIn _ Î)) (punchesIn Î Ïƒ x)
    â‰¡âŸ¨âŸ©
  rename ((punchIn _ (Î , C)) âˆ˜ S_) (punchesIn Î Ïƒ x)
    â‰¡âŸ¨ sym (rename-comp S_ (punchIn _ (Î , C))) âŸ©
  rename (punchIn _ (Î , C)) (rename S_ (punchesIn Î Ïƒ x))
    âˆ
  where open PropEq.â‰¡-Reasoning

punchIn-punchesIn-comm : (Ïƒ : Subst Î“ Î”)
  â†’ (M : Î“ â§º Î âŠ¢ A)
  â†’ rename (punchIn B Î) M âŸª punchesIn Î (exts Ïƒ) âŸ«
   â‰¡ rename (punchIn B Î) (M âŸª punchesIn Î Ïƒ âŸ«)
punchIn-punchesIn-comm Ïƒ (` x)      = punchesIn-punchIn-comm Ïƒ x
--punchIn-punchesIn-comm Ïƒ (absurd A M) = cong (absurd A) (punchIn-punchesIn-comm Ïƒ M)
punchIn-punchesIn-comm Ïƒ (M Â· N)    = congâ‚‚ _Â·_ (punchIn-punchesIn-comm Ïƒ M) (punchIn-punchesIn-comm Ïƒ N)
punchIn-punchesIn-comm Ïƒ (Æ› M) = cong Æ›_ (begin
  rename (ext (punchIn _ _)) M âŸª exts (punchesIn _ (exts Ïƒ)) âŸ«
    â‰¡âŸ¨ cong _âŸª exts (punchesIn _ (exts Ïƒ)) âŸ« (rename-cong ext-punchIn=punchIn M) âŸ©
  rename (punchIn _ (_ , _)) M âŸª exts (punchesIn _ (exts Ïƒ)) âŸ«
    â‰¡âŸ¨ subst-cong exts-punchesIn=punchesIn (rename (punchIn _ (_ , _)) M) âŸ©
  rename (punchIn _ (_ , _)) M âŸª punchesIn (_ , _) (exts Ïƒ) âŸ«
    â‰¡âŸ¨ punchIn-punchesIn-comm Ïƒ M âŸ©
  rename (punchIn _ (_ , _)) (M âŸª punchesIn (_ , _) Ïƒ âŸ«)
    â‰¡âŸ¨ rename-cong (sym âˆ˜ ext-punchIn=punchIn) (M âŸª punchesIn (_ , _) Ïƒ âŸ«) âŸ©
  rename (ext (punchIn _ _)) (M âŸª punchesIn (_ , _) Ïƒ âŸ«)
    â‰¡âŸ¨ cong (rename (ext (punchIn _ _))) (subst-cong (sym âˆ˜ exts-punchesIn=punchesIn) M) âŸ©
  rename (ext (punchIn _ _)) (M âŸª exts (punchesIn _ Ïƒ) âŸ«)
    âˆ)
  where open PropEq.â‰¡-Reasoning

rename-exts : (Ïƒ : Subst Î“ Î”)
  â†’ (M : Î“ âŠ¢ A)
  â†’ rename (S_ {B = B}) M âŸª exts Ïƒ âŸ« â‰¡ rename S_ (M âŸª Ïƒ âŸ«)
rename-exts Ïƒ M = begin
  rename S_ M âŸª exts Ïƒ âŸ«
    â‰¡âŸ¨ cong _âŸª exts Ïƒ âŸ« (rename-cong S=punchIn M) âŸ©
  rename (punchIn _ âˆ…) M âŸª punchesIn âˆ… (exts Ïƒ) âŸ«
    â‰¡âŸ¨ punchIn-punchesIn-comm Ïƒ M âŸ©
  rename (punchIn _ âˆ…) (M âŸª Ïƒ âŸ«)
    â‰¡âŸ¨ rename-cong (sym âˆ˜ S=punchIn) (M âŸª Ïƒ âŸ«) âŸ©
  rename S_ (M âŸª Ïƒ âŸ«)
    âˆ 
  where open PropEq.â‰¡-Reasoning

ren-ext-comm : (Ï : Rename Î“ Î”)
    â†’ (x : Î“ , B âˆ‹ A)
    â†’ ren (ext Ï) x â‰¡ exts (ren Ï) x
ren-ext-comm Ï Z     = refl
ren-ext-comm Ï (S _) = refl

----------------------------------------------------------------------
-- Monad Laws 

subst-idR : (Ïƒ : Subst Î“ Î”) {x : Î“ âˆ‹ A}
  â†’ ` x âŸª Ïƒ âŸ« â‰¡ Ïƒ x
subst-idR Ïƒ = refl

subst-idL
  : (M : Î“ âŠ¢ A)
  â†’ M âŸª ids âŸ« â‰¡ M
subst-idL (` x)      = refl
--subst-idL (absurd A M) = cong (absurd A) (subst-idL M)
subst-idL (M Â· N)    = congâ‚‚ _Â·_    (subst-idL M) (subst-idL N)
subst-idL (Æ›_ M)     = begin
  Æ› M âŸª exts ids âŸ« 
    â‰¡âŸ¨ cong Æ›_ (subst-cong exts-ids=ids M) âŸ© 
  Æ› M âŸª ids âŸ«
    â‰¡âŸ¨ cong Æ›_ (subst-idL M) âŸ©
  Æ› M  âˆ
  where
    open PropEq.â‰¡-Reasoning
    exts-ids=ids : (x : Î“ , A âˆ‹ B) â†’ (exts ids) x â‰¡ ids x
    exts-ids=ids Z     = refl
    exts-ids=ids (S x) = refl

subst-assoc
  : (Ïƒâ‚ : Subst Î“ Î”) (Ïƒâ‚‚ : Subst Î” Î)
  â†’ (M : Î“ âŠ¢ A)
  â†’  M âŸª Ïƒâ‚ âŸ« âŸª Ïƒâ‚‚ âŸ« â‰¡ M âŸª Ïƒâ‚ â¨Ÿ Ïƒâ‚‚ âŸ«
subst-assoc Ïƒâ‚ Ïƒâ‚‚ (` x)      = refl
--subst-assoc Ïƒâ‚ Ïƒâ‚‚ (absurd A M) = cong (absurd A) (subst-assoc Ïƒâ‚ Ïƒâ‚‚ M)
subst-assoc Ïƒâ‚ Ïƒâ‚‚ (M Â· N)    = congâ‚‚ _Â·_ (subst-assoc Ïƒâ‚ Ïƒâ‚‚ M) (subst-assoc Ïƒâ‚ Ïƒâ‚‚ N)
subst-assoc Ïƒâ‚ Ïƒâ‚‚ (Æ› M)      = cong  Æ›_ (begin
  M âŸª exts Ïƒâ‚ âŸ« âŸª exts Ïƒâ‚‚ âŸ« 
    â‰¡âŸ¨ subst-assoc (exts Ïƒâ‚) (exts Ïƒâ‚‚) M âŸ©
  M âŸª _âŸª exts Ïƒâ‚‚ âŸ« âˆ˜ exts Ïƒâ‚ âŸ«
    â‰¡âŸ¨ subst-cong (exts-subst Ïƒâ‚ Ïƒâ‚‚) M âŸ©
  M âŸª exts ( _âŸª Ïƒâ‚‚ âŸ« âˆ˜ Ïƒâ‚) âŸ«
    âˆ)
  where
    open PropEq.â‰¡-Reasoning
    exts-subst : (Ïƒâ‚ : Subst Î“ Î”) (Ïƒâ‚‚ : Subst Î” Î)
      â†’ (x : Î“ , B âˆ‹ A) 
      â†’ (exts Ïƒâ‚ â¨Ÿ exts Ïƒâ‚‚) x â‰¡ exts (Ïƒâ‚ â¨Ÿ Ïƒâ‚‚) x
    exts-subst Ïƒâ‚ Ïƒâ‚‚ Z     = refl
    exts-subst Ïƒâ‚ Ïƒâ‚‚ (S x) = begin
      (exts Ïƒâ‚ â¨Ÿ exts Ïƒâ‚‚) (S x)
        â‰¡âŸ¨âŸ©
      rename S_ (Ïƒâ‚ x) âŸª exts Ïƒâ‚‚ âŸ« 
        â‰¡âŸ¨ rename-exts Ïƒâ‚‚ (Ïƒâ‚ x)  âŸ©
      rename S_ (Ïƒâ‚ x âŸª Ïƒâ‚‚ âŸ«)
        â‰¡âŸ¨âŸ©
      exts (Ïƒâ‚ â¨Ÿ Ïƒâ‚‚) (S x)
        âˆ

----------------------------------------------------------------------
-- 

rename-subst : (Ï : Rename Î“ Î”) (Ïƒ : Subst Î” Î)
  â†’ (M : Î“ âŠ¢ A)
  â†’  rename Ï M âŸª Ïƒ âŸ« â‰¡ M âŸª Ïƒ âˆ˜ Ï âŸ«
rename-subst Ï Ïƒ M = begin
  (rename Ï M) âŸª Ïƒ âŸ« 
    â‰¡âŸ¨ cong _âŸª Ïƒ âŸ« (rename=subst-ren M) âŸ©
  (M âŸª ren Ï âŸ«) âŸª Ïƒ âŸ« 
    â‰¡âŸ¨ subst-assoc (ren Ï) Ïƒ M âŸ©
  M âŸª ren Ï â¨Ÿ Ïƒ âŸ«
    â‰¡âŸ¨âŸ©
  M âŸª Ïƒ âˆ˜ Ï âŸ«
    âˆ
  where open PropEq.â‰¡-Reasoning

subst-zero-comm : (Ïƒ : Subst Î“ Î”)
  â†’ (N : Î“ âŠ¢ B) (x : Î“ , B âˆ‹ A)
  â†’ (exts Ïƒ â¨Ÿ subst-zero (N âŸª Ïƒ âŸ«)) x â‰¡ (subst-zero N â¨Ÿ Ïƒ) x
subst-zero-comm         Ïƒ N Z     = refl
subst-zero-comm {Î“} {Î”} Ïƒ N (S x) = begin
  (rename S_ (Ïƒ x)) âŸª subst-zero (N âŸª Ïƒ âŸ«) âŸ« 
    â‰¡âŸ¨ cong (_âŸª subst-zero (N âŸª Ïƒ âŸ«) âŸ«) (rename=subst-ren (Ïƒ x)) âŸ©
  Ïƒ x âŸª ren S_ âŸ« âŸª subst-zero (N âŸª Ïƒ âŸ«) âŸ« 
    â‰¡âŸ¨ subst-assoc (ren S_) (subst-zero (N âŸª Ïƒ âŸ«)) (Ïƒ x) âŸ©
  Ïƒ x âŸª subst-zero (N âŸª Ïƒ âŸ«) âˆ˜ S_ âŸ« 
    â‰¡âŸ¨ refl âŸ©
  Ïƒ x âŸª ids âŸ« 
    â‰¡âŸ¨ subst-idL (Ïƒ x) âŸ©
  Ïƒ x
    âˆ
  where open PropEq.â‰¡-Reasoning

------------------------------------------------------------------------------
-- Substitution Lemma

subst-ssubst : (Ïƒ : Subst Î“ Î”)
  â†’ (M : Î“ , A âŠ¢ B) (N : Î“ âŠ¢ A)
  â†’ M âŸª exts Ïƒ âŸ« [ N âŸª Ïƒ âŸ« ] â‰¡ M [ N ] âŸª Ïƒ âŸ« 
subst-ssubst Ïƒ M N = begin
  M âŸª exts Ïƒ âŸ« [ N âŸª Ïƒ âŸ« ]
    â‰¡âŸ¨ subst-assoc (exts Ïƒ) (subst-zero (N âŸª Ïƒ âŸ«)) M âŸ©
  M âŸª exts Ïƒ â¨Ÿ subst-zero (N âŸª Ïƒ âŸ«) âŸ«
    â‰¡âŸ¨ subst-cong (subst-zero-comm Ïƒ N) M âŸ© 
  M âŸª subst-zero N â¨Ÿ Ïƒ âŸ«
    â‰¡âŸ¨ sym (subst-assoc (subst-zero N) Ïƒ M) âŸ©
  (M âŸª subst-zero N âŸ«) âŸª Ïƒ âŸ« 
    âˆ
  where open PropEq.â‰¡-Reasoning

rename-ssubst : (Ï : Rename Î“ Î”)
  â†’ (M : Î“ , A âŠ¢ B) (N : Î“ âŠ¢ A)
  â†’ rename (ext Ï) M [ rename Ï N ] â‰¡ rename Ï (M [ N ])
rename-ssubst Ï M N = begin
  rename (ext Ï) M [ rename Ï N ]
    â‰¡âŸ¨ cong (_âŸª subst-zero (rename Ï N) âŸ«) (rename=subst-ren M) âŸ©
  M âŸª ren (ext Ï) âŸ« âŸª subst-zero (rename Ï N) âŸ«
    â‰¡âŸ¨ cong _âŸª subst-zero (rename Ï N) âŸ« (subst-cong (ren-ext-comm Ï) M) âŸ©
  M âŸª exts (ren Ï) âŸ« âŸª subst-zero (rename Ï N) âŸ«
    â‰¡âŸ¨ subst-cong (Î» { Z â†’ rename=subst-ren N ; (S x) â†’ refl}) (M âŸª exts (ren Ï) âŸ«) âŸ©
  M âŸª exts (ren Ï) âŸ« [ N âŸª ren Ï âŸ« ]
    â‰¡âŸ¨ subst-ssubst (ren Ï) M N âŸ©
  M [ N ] âŸª ren Ï âŸ«
    â‰¡âŸ¨ sym (rename=subst-ren _) âŸ©
  rename Ï (M [ N ])
    âˆ
  where
    open PropEq.â‰¡-Reasoning

------------------------------------------------------------------------------
-- Substitution respects reduction

rename-reduce : {Ï : Rename Î“ Î”}
  â†’ M -â†’ N
  â†’ rename Ï M -â†’ rename Ï N
rename-reduce {Ï = Ï} (Î²-Æ›Â· {M = M} {N})
  rewrite PropEq.sym (rename-ssubst Ï M N) = Î²-Æ›Â· 
--rename-reduce (Î¾-absurd M-â†’N) = Î¾-absurd (rename-reduce M-â†’N)
rename-reduce (Î¾-Æ› M-â†’N)      = Î¾-Æ› (rename-reduce  M-â†’N)
rename-reduce (Î¾-Â·â‚— M-â†’N)     = Î¾-Â·â‚— (rename-reduce M-â†’N)
rename-reduce (Î¾-Â·áµ£ M-â†’N)     = Î¾-Â·áµ£ (rename-reduce M-â†’N)

subst-reduce : {Ïƒ : Subst Î“ Î”}
  â†’ M -â†’ N
  â†’ M âŸª Ïƒ âŸ« -â†’ N âŸª Ïƒ âŸ«
subst-reduce {Ïƒ = Ïƒ} (Î²-Æ›Â· {M = M} {N})
  rewrite PropEq.sym (subst-ssubst Ïƒ M N) = Î²-Æ›Â·
--subst-reduce (Î¾-absurd M-â†’N) = Î¾-absurd (subst-reduce M-â†’N)
subst-reduce (Î¾-Æ› M-â†’N)  = Î¾-Æ›  (subst-reduce M-â†’N)
subst-reduce (Î¾-Â·â‚— M-â†’N) = Î¾-Â·â‚— (subst-reduce M-â†’N)
subst-reduce (Î¾-Â·áµ£ M-â†’N) = Î¾-Â·áµ£ (subst-reduce M-â†’N)
